src/program_proof/mpaxos/applyasfollower_proof.v
@@ -43,7 +43,108 @@ Lemma wp_singleClerk__applyAsFollower ck γ γsrv σ Q args_ptr args :
                                                    True
   }}}.
 Proof.
-Admitted.
+  iIntros (Φ) "Hpre HΦ".
+  iNamed "Hpre".
+  wp_call.
+  wp_apply (applyAsFollowerArgs.wp_Encode with "Hargs").
+  iIntros (enc enc_sl) "[%Hargs_enc Hsl]".
+  wp_pures.
+  wp_apply (wp_ref_of_zero).
+  { done. }
+  iIntros (rep_ptr) "Hrep".
+  wp_pures.
+  iNamed "His_ck".
+  wp_loadField.
+  iDestruct (is_slice_to_small with "Hsl") as "Hsl".
+  iApply (wp_frame_wand with "[HΦ]").
+  { iNamedAccu. }
+  wp_apply (wp_ReconnectingClient__Call2 with "Hcl_rpc [] Hsl Hrep").
+  {
+    unfold is_mpaxos_host.
+    iNamed "Hsrv".
+    iFrame "#".
+  }
+  { (* Successful RPC *)
+    iModIntro.
+    iNext.
+    unfold enterNewEpoch_spec.
+    iExists _, _, _.
+    iSplitR; first done.
+    iSplit.
+    {
+      instantiate (1:=σ).
+      unfold get_state.
+      rewrite fmap_last.
+      rewrite Hghost_op_σ.
+      simpl.
+      done.
+    }
+    iFrame "%#".
+
+    iSplit.
+    {
+      iIntros "#Hacc_lb".
+      iIntros (?) "%Henc_reply Hsl".
+      iIntros (?) "Hrep Hrep_sl".
+      wp_pures.
+      wp_load.
+      rewrite Henc_reply.
+      wp_apply (applyAsFollowerReply.wp_Decode with "[$Hrep_sl]").
+      { done. }
+      iIntros (reply_ptr) "Hreply".
+      iIntros "HΦ".
+      iApply "HΦ".
+      iFrame "∗".
+      destruct (decide _).
+      { iModIntro. iFrame "#". }
+      done.
+    }
+    { (* Apply failed for some reason, e.g. node is not primary *)
+      iIntros (? Hreply_err).
+      iIntros (?) "%Henc_reply Hsl".
+      iIntros (?) "Hrep Hrep_sl".
+      wp_pures.
+      wp_load.
+      rewrite Henc_reply.
+      wp_apply (applyAsFollowerReply.wp_Decode with "[$Hrep_sl]").
+      { done. }
+      iIntros (reply_ptr) "Hreply".
+      iIntros "HΦ".
+      iApply "HΦ".
+      iFrame "∗".
+      destruct (decide _).
+      { exfalso. done. }
+      { done. }
+    }
+  }
+  { (* RPC error *)
+    iIntros.
+    wp_pures.
+    destruct (bool_decide _) as [] eqn:X.
+    {
+      exfalso.
+      apply bool_decide_eq_true in X.
+      naive_solver.
+    }
+    wp_pures.
+
+    wp_apply (wp_allocStruct).
+    { repeat econstructor. }
+    iIntros (reply_ptr) "Hreply".
+    iNamed 1.
+    iApply "HΦ".
+    iDestruct (struct_fields_split with "Hreply") as "HH".
+    iNamed "HH".
+
+    iSplitL.
+    {
+      instantiate (1:=applyAsFollowerReply.mkC _).
+      iFrame "∗#".
+    }
+    simpl.
+    done.
+  }
+Qed.
 
 Lemma wp_Server__applyAsFollower (s:loc) (args_ptr reply_ptr:loc) γ γsrv args init_reply σ Q Φ Ψ :
   is_Server conf s γ γsrv -∗
